theories/VLSM/Core/Composition.v
@@ -687,7 +687,8 @@ Lemma [basic_VLSM_incl]
       - intro; intros. apply lift_to_composite_state_initial. assumption.
     Qed.
 
-    (** If all messages desribed by a predicate <<P>> are valid for the free
+    (**
+    If all messages desribed by a predicate <<P>> are valid for the free
     composition pre-loaded with messages described by a predicate <<Q>>, then
     any message which can be emitted by a component pre-loaded with <<P>> can
     also be emitted by the free composition pre-loaded with <<Q>>.
@@ -707,7 +708,8 @@ Lemma [basic_VLSM_incl]
         intuition.
     Qed.
 
-    (** As a specialization of [valid_preloaded_lifts_can_be_emitted], if all
+    (**
+    As a specialization of [valid_preloaded_lifts_can_be_emitted], if all
     messages desribed by a predicate <<P>> are valid for the free composition,
     then any message which can be emitted by a component pre-loaded with <<P>>
     can also be emitted by the free composition.
